template-coq/src/reification.ml
@@ -36,9 +36,6 @@ sig
   type quoted_mind_finiteness
   type quoted_entry
 
-  type quoted_recarg
-  type quoted_wf_paths
-
   (* Local contexts *)
   type quoted_context_decl
   type quoted_context
