template-coq/theories/Ast.v
@@ -1,7 +1,6 @@
 (* Distributed under the terms of the MIT license. *)
 From MetaCoq.Template Require Import utils Environment.
 From MetaCoq.Template Require Export Universes.
-Export utils.MCRTree.
 
 
 
